defined a module type for GenericValue, such that in Coq, it is instantiated by CompCert.Mem; while extracting, it is implemented by the LLVM interperter mem manager; connected extracted generic value functions with LLVM.
git-svn-id: https://webdav.seas.upenn.edu/svn/sol/vol@2692 eef5ea85-cc2e-0410-bd84-0fae1f012da8

src/ssa/extraction/Llvmcaml.ml
@@ -1,31 +1,70 @@
 open Llvm_executionengine
 open Ssa_def
+open LLVMsyntax
+
+let coqtype_2_llvmtype (t:LLVMsyntax.typ) : Llvm.lltype = failwith "undef"
+let coqbop_2_llvmopcode (op:LLVMsyntax.bop) : Llvm.InstrOpcode.t = failwith "undef"
+let coqtd_2_llvmtd (td:layouts) : Llvm_target.TargetData.t = failwith "undef"
+let coqcond_2_llvmicmp (c:cond) : Llvm.Icmp.t = failwith "undef"
 
 module GenericValue = struct
 
   type t = GenericValue.t
 
+  (* useless at runtime *)
   let null = failwith "undef"
-
   let sizeGenericValue x = failwith "undef"
   let uninits x = failwith "undef"
   let gv2val x y = failwith "undef"
   let gv2int x y z = failwith "undef"
   let gv2ptr x y z = failwith "undef"
-  let val2GV x y z = failwith "undef"
-  let ptr2GV x y = failwith "undef"
-  let blk2GV x = failwith "undef"
-  let mgep x y z w = failwith "undef"
+  let val2gv x y z = failwith "undef"
+  let ptr2gv x y = failwith "undef"
   let _const2GV x y z = failwith "undef"
   let _list_const_arr2GV x y z = failwith "undef" 
   let _list_const_struct2GV x y z = failwith "undef" 
-  let const2GV x y z = failwith "undef"
+
+  (* used at runtime *)
+  let blk2gv (td:LLVMsyntax.layouts) (v:t) = v
+
+  let isZero (td:LLVMsyntax.layouts) (v:t) = GenericValue.as_int v == 0
+
+  let const2GV (td:LLVMsyntax.layouts) gl (c:LLVMsyntax.const) : t option = 
+    failwith "undef"
+
+  let mgep x y z w = failwith "undef"
+
   let extractGenericValue x y z w = failwith "undef"
+
   let insertGenericValue x y z a b = failwith "undef"
-  let mbop x y z a b = failwith "undef"
-  let mcast x y z a b = failwith "undef"
-  let mext x y z a b = failwith "undef"
-  let micmp x y z a b = failwith "undef"
+
+  let mbop (td:LLVMsyntax.layouts) (op:LLVMsyntax.bop) (bsz:LLVMsyntax.sz) (gv1:t) (gv2:t) = 
+    Some (GenericValue.binary_op gv1 gv2 (Llvm.integer_type (Llvm.global_context()) bsz) (coqbop_2_llvmopcode op))
+
+  let mcast (td:LLVMsyntax.layouts) (op:LLVMsyntax.castop) (t1:LLVMsyntax.typ) (gv1:t) (t2:LLVMsyntax.typ) =
+  Some(
+  match op with
+    | Coq_castop_fptoui -> GenericValue.fptoui gv1 (coqtype_2_llvmtype t1) (coqtype_2_llvmtype t2)
+    | Coq_castop_fptosi -> GenericValue.fptosi gv1 (coqtype_2_llvmtype t1) (coqtype_2_llvmtype t2)
+    | Coq_castop_uitofp -> GenericValue.uitofp gv1 (coqtype_2_llvmtype t2)
+    | Coq_castop_sitofp -> GenericValue.sitofp gv1 (coqtype_2_llvmtype t2)
+    | Coq_castop_ptrtoint -> GenericValue.ptrtoint gv1 (coqtype_2_llvmtype t1) (coqtype_2_llvmtype t2)
+    | Coq_castop_inttoptr -> GenericValue.inttoptr (coqtd_2_llvmtd td) gv1 (coqtype_2_llvmtype t2)
+    | Coq_castop_bitcast -> GenericValue.bitcast gv1 
+                              (coqtype_2_llvmtype t1) 
+                              (Llvm.global_context()) 
+                              (coqtype_2_llvmtype t2)
+  )
+
+  let mext (td:layouts) (op:extop) (t1:typ) (gv1:t) (t2:typ) =
+  Some(
+  match op with
+    | Coq_extop_z -> GenericValue.zext gv1 (coqtype_2_llvmtype t2)
+    | Coq_extop_s -> GenericValue.sext gv1 (coqtype_2_llvmtype t2)
+  )
+
+  let micmp (td:layouts) (c:cond) (t:typ) (gv1:t) (gv2:t) =
+  Some (GenericValue.icmp gv1 gv2 (coqtype_2_llvmtype t) (coqcond_2_llvmicmp c))
 
 end
 
@@ -45,8 +84,6 @@ module Mem = struct
     let (ee, _) = m in
     let _ = ExecutionEngine.free_memory ptr ee in
     Some m
-
-  let coqtype_2_llvmtype t = failwith "undef"
 
   let mload (td:LLVMsyntax.layouts) m ptr t (a:LLVMsyntax.align) =
     let (ee, _) = m in
