src/ssa/ssa_coq_lib.v
@@ -593,6 +593,17 @@ match b with
 | (block_intro _ lp _ _) => lp
 end.
 
+Definition getEntryBlock (fd:fdef) : option block :=
+match fd with
+| fdef_intro _ (b::_) => Some b
+| _ => None
+end.
+
+Definition getEntryCmds (b:block) : cmds :=
+match b with
+| block_intro _ _ lc _ => lc
+end.
+
 (**********************************)
 (* Lookup. *)
 
